TransVal/transval.v
@@ -1,5 +1,5 @@
-Require Import List Specif.
-Require Import IL Annotation AutoIndTac Bisim Exp MoreExp Coherence Fresh sexp smt.
+Require Import List.
+Require Import IL Annotation AutoIndTac Bisim Exp MoreExp Coherence Fresh sexp smt nofun.
 
 Definition wrapEnv E :=
 fun (x:var) =>
@@ -13,7 +13,8 @@ Lemma models_if_eval :
 forall s D E s' E' , 
 ssa  s D
 -> star2 step (nil, E,s) nil (nil, E',s')
--> forall p, models (wrapEnv E)  (translateStmt s p).
+(*-> s' = f e \/ s' = e *)
+-> forall p, models (wrapEnv E')  (translateStmt s p).
 
 Proof.
 admit.
@@ -24,8 +25,6 @@ smtAnd (translateStmt s source) (translateStmt t target).
 
 (** TODO: Why doesn't this work? **)
 Fixpoint agreeOnList (E:senv) (XL:list var) (YL:list var):=
-True.
-(*
 match XL, YL with
 |nil , nil => True
 | nil, _ => False
@@ -34,15 +33,14 @@ match XL, YL with
                         | Some v1, Some v2 => v1 = v2 /\ (agreeOnList E XL' YL')
                         | None, None =>  (agreeOnList E XL' YL')
                         | _,_ => False
-                    end
-end. *)
+                    end.
 
 (** TODO: Add constraint that XL and YL are the lists of the output variables of the corresponding programs **)
 Lemma not_smtCheck_entails_sat:
 forall s t E XL YL,
 ~ (models E (smtCheck s t))
 -> (forall p V,  models V (translateStmt s p) -> models V (translateStmt s p))
--> agreeOnList E XL YL.
+-> agree_on E XL YL.
 
 Proof.
 admit.
@@ -54,6 +52,7 @@ forall s t s' t' E E1 E2 x y,
 (star2 step (nil, E , s) nil (nil, E1, s'))
 -> (star2 step (nil, E, t) nil (nil, E2, t'))
 -> E1 x = E2 y.
+
 (*
 *** Local Variables: ***
 *** coq-load-path: (("../" "Lvc")) ***
